updated q2

A1/Q2.dfy
@@ -3,49 +3,23 @@ requires a != null;
 requires 0 <= min <= max <= a.Length;
 reads a;
 {
-  forall j, k :: min <= j < k < max ==> a[j] <= a[k]
+    forall j, k :: min <= j < k < max ==> a[j] <= a[k]
 }
 
- method max (a: array<int>) returns (max: nat)
-  requires a != null && a.Length > 0;
-  ensures forall j:: 0 <= j < a.Length ==> a[j] <= max;
-  ensures exists j:: 0 <= j < a.Length && a[j] == max;
+function min (a: array<int>, left: int, right: int): int
+    requires a != null && a.Length > 0;
+    requires 0 < left <= right < a.Length;
+    reads a;
 {
-  max := 0;
-  var i := 0;
-
-  while (i < a.Length)
-    invariant 0 <= i <= a.Length;
-    invariant forall j:: 0<=j<i ==> a[j] <= max;
-    invariant i!=0 ==> exists j:: 0<=j<i && a[j]==max;
-    invariant i==0 ==> a[0] >= max;
-  {
-    if (a[i] > max) {
-      max := a[i]; 
-    }
-    i := i + 1;
-  }
+    if (a[left] > a[right]) then a[right] else a[left]
 }
 
- method min (a: array<int>) returns (max: nat)
-  requires a != null && a.Length > 0;
-  ensures forall j:: 0<=j<a.Length ==> a[j] <= max;
-  ensures exists j:: 0<=j<a.Length && a[j]==max;
+function max (a: array<int>, left: int, right: int): int
+    requires a != null && a.Length > 0;
+    requires 0 < left <= right < a.Length;
+    reads a;
 {
-  max := 0;
-  var i := 0;
-
-  while (i < a.Length)
-    invariant 0 <= i <= a.Length;
-    invariant forall j:: 0<=j<i ==> a[j] <= max;
-    invariant i!=0 ==> exists j:: 0<=j<i && a[j]==max;
-    invariant i==0 ==> a[0] >= max;
-  {
-    if (a[i] > max) {
-      max := a[i]; 
-    }
-    i := i + 1;
-  }
+    if (a[left] > a[right]) then a[left] else a[right]
 }
 
 method stoogeSort(a: array <int>, left: int, right: int) 
@@ -55,10 +29,10 @@ method stoogeSort(a: array <int>, left: int, right: int)
     modifies a;
     ensures sorted(a, left, right);
     ensures forall i :: (0 <= i < left || right < i < a.Length) ==> a[i] == old(a[i]);
-    //ensures a[left] == min(a,left,right);
-    //ensures a[right] == max(a,left,right);
-    //ensures min(a, left, right) == old(min(a, left, right));
-    //ensures max(a, left, right) == old(max(a, left, right));
+    ensures a[left] == min(a,left,right);
+    ensures a[right] == max(a,left,right);
+    ensures min(a, left, right) == old(min(a, left, right));
+    ensures max(a, left, right) == old(max(a, left, right));
 {
     if (a[left] > a[right]) {
         // swap a[left] and a[right]
@@ -75,3 +49,70 @@ method stoogeSort(a: array <int>, left: int, right: int)
     stoogeSort(a, left, right - k); // First two-thirds again
 }
 
+
+
+// method max (a: array<int>) returns (max: nat)
+//     requires a != null && a.Length > 0;
+//     ensures forall j:: 0 <= j < a.Length ==> a[j] <= max;
+//     ensures exists j:: 0 <= j < a.Length && a[j] == max;
+// {
+//     max := 0;
+//     var i := 0;
+
+//     while (i < a.Length)
+//         invariant 0 <= i <= a.Length;
+//         invariant forall j:: 0<=j<i ==> a[j] <= max;
+//         invariant i!=0 ==> exists j:: 0<=j<i && a[j]==max;
+//         invariant i==0 ==> a[0] >= max;
+//     {
+//         if (a[i] > max) {
+//             max := a[i]; 
+//         }
+//         i := i + 1;
+//     }
+// }
+
+// method min (a: array<int>) returns (max: nat)
+//     requires a != null && a.Length > 0;
+//     ensures forall j:: 0<=j<a.Length ==> a[j] <= max;
+//     ensures exists j:: 0<=j<a.Length && a[j]==max;
+// {
+//     max := 0;
+//     var i := 0;
+
+//     while (i < a.Length)
+//         invariant 0 <= i <= a.Length;
+//         invariant forall j:: 0<=j<i ==> a[j] <= max;
+//         invariant i!=0 ==> exists j:: 0<=j<i && a[j]==max;
+//         invariant i==0 ==> a[0] >= max;
+//     {
+//         if (a[i] > max) {
+//             max := a[i]; 
+//         }
+//         i := i + 1;
+//     }
+// }
+
+// method min (a: array<int>, left: int, right: int) returns (min: int)
+//     requires a != null && a.Length > 0;
+//     requires left <= right <= a.Length;
+//     ensures a[left] <= a[right];
+// {
+//     if (a[left] > a[right]) {
+//         min := a[right];
+//     } else {
+//         min := a[left];
+//     }
+// }
+
+//  method max (a: array<int>, left: int, right: int) returns (max: int)
+//     requires a != null && a.Length > 0;
+//     requires left <= right <= a.Length;
+//     ensures a[left] <= a[right];
+// {
+//     if (a[left] > a[right]) {
+//         max := a[left];
+//     } else {
+//         max := a[right];
+//     }
+// }
